monadproofs/proofs/demoprf.v
@@ -4,81 +4,25 @@ Require Import monad.proofs.libspecs.
 Require Import bedrock.auto.invariants.
 Require Import bedrock.auto.cpp.proof.
 Require Import bedrock.auto.cpp.tactics4.
+Require Import monad.proofs.demomisc.
 Import cQp_compat.
 Open Scope cQp_scope.
+Import Verbose.
 Section with_Sigma.
   Context `{Sigma:cpp_logic} {CU: genv}.
   Context  {MODd : demo.module ⊧ CU}.
   Definition cQpc := cQp.mk false.
   Coercion cQpc : Qp >-> cQp.t.
 
-  Arguments primR.body {thread_info _Σ Σ σ} ty%cpp_type_scope q%cQp_scope v.
   cpp.spec "foo()" as foo_spec with (
-        \prepost{xv:N} _global "x" |-> primR "unsigned int" 1 xv
-        \pre{yv:N} _global "y" |-> primR.body "unsigned int" 1 yv
-        \post _global "y" |-> primR.body "unsigned int" 1 (xv+1)%N
+        \prepost{xv:N} _global "x" |-> primR "unsigned int" 1  xv
+        \pre{yv:N} _global "y" |-> primR "unsigned int" 1 yv
+        \post _global "y" |-> primR "unsigned int" 1 (xv+1)%N
       ).
 
-
-  Import Verbose.
-      Ltac hideLoc l :=
-        IPM.perm_left ltac:(fun t n=>
-                              match t with
-                              | l |-> ?r => hideFromWork r
-                              end
-
-                           ).
-
-      Lemma primR_anyR_ex: ∀  (t : type) (q : cQp.t),
-         Exists v,  primR t q v ⊢ anyR t q.
-      Proof using.
-        intros.
-        go.
-      Qed.
-
-  Lemma uncurry_post_wand (P:mpred) (Qs Q: ptr -> mpred):
-    (P -* Forall x, (Qs x-* Q x))
-      |-- (Forall x, ((P ** Qs x)-* Q x)).
-  Proof. Admitted.
-    Lemma wpl f ρ s Qs Q:
-      (Forall v, Qs v -* Q v) **  (wp f ρ s (Kreturn (λ v : ptr, Qs v))) |--
-        (wp f ρ s (Kcleanup module [] (Kreturn (λ v : ptr, |> Q v)))).
-    Proof using. Admitted.
-
-  Ltac clearPost :=
-    repeat match goal with
-    | H: mpred |- _ => try clear H
-    | H : ptr-> mpred |- _ => try clear H
-    end.
-    
-  Ltac verify_spec2 :=
-    work; (* NOT go as that puts Seq into the continuation as Kseq, making the next rewrite fail *)
-    try rewrite uncurry_post_wand; (* TODO: make it work only the hyp of the form -* POST v *)
-    rewrite <- wpl;
-    eagerUnifyU; (* this does not suffice: see split_spec proof. need to do evar tricks to infer Qs *)
-    work;
-    name_locals;
-    cpp.hints.type.has_type_prop_prep;
-    try clearPost.
-      
-  Ltac verify_spec1 :=
-    iApply (verify_spec_new false false false module with ""%string);
-    [vm_compute; reflexivity|].
-
-  Ltac verify_spec :=
-    iIntrosDestructs;
-    verify_spec1;
-    verify_spec2.
-
-      Ltac runUntilPost :=
-      match goal with
-        |- context[Kreturn ?post] => hideFromWork post
-      end;
-      go;
-      unhideAllFromWork;
-      repeat rewrite <- primR_tptsto_fuzzyR.
   Lemma prf: denoteModule demo.module |-- foo_spec.
   Proof using.
+    iIntrosDestructs.
     verify_spec.
     do 5 run1.
     - slauto.
@@ -104,10 +48,13 @@ Section with_Sigma.
     verify_spec'.
     slauto.
   Qed.
+
+
+  
   cpp.spec "sfoo()" as sfoo_spec with (
         \prepost{xv:Z} _global "a" |-> primR "int" 1 xv
         \pre{yv:N} _global "b" |-> primR.body "int" 1 yv
-        \post _global "b" |-> primR.body "int" 1 ((xv+1) `mod` (2^32))%Z
+        \post _global "b" |-> primR.body "int" 1 ((xv+1))%Z
       ).
 
   Lemma sprf: denoteModule demo.module |-- sfoo_spec.
@@ -131,5 +78,123 @@ Section with_Sigma.
     slauto.
   Qed.
 
+
+  Definition ThreadR (lamStructName: core.name) (P Q : mpred) : Rep. Proof using. Admitted.
+  
+  Definition ThreadConstructor (lamStructName: core.name) (this:ptr): WpSpec mpredI val val :=
+    \arg{lambdap:ptr} "lambda" (Vref lambdap)
+    \pre{lamStructObjOwnership} lambdap |-> lamStructObjOwnership (* ownerhsip of fields othe lambda struct *)
+    \pre{taskPre taskPost}
+      specify {| info_name :=  (Nscoped lamStructName taskOpName);
+                info_type := tMethod lamStructName QC "void" [] |}
+      (fun (this:ptr) =>
+         \prepost this |-> lamStructObjOwnership
+         \pre taskPre
+         \post taskPost)
     
+    \post this |-> ThreadR lamStructName taskPre taskPost.
+
+  Definition fork_start (lamStructName: core.name) (this:ptr): WpSpec mpredI val val :=
+    \prepost{P Q} this |-> ThreadR lamStructName P Q
+    \pre P
+    \post emp.
+
+  Definition join (lamStructName: core.name) (this:ptr): WpSpec mpredI val val :=
+    \prepost{P Q} this |-> ThreadR lamStructName P Q
+    \post Q.
+
+  cpp.spec "parallel_gcd_lcm(const unsigned int&, const unsigned int&, unsigned int&, unsigned int&)" as pgl with
+      (
+        \arg{ap} "a" (Vref ap)
+        \prepost{(qa:Qp) (av:N)} ap |-> primR "int" qa av
+        \arg{bp} "b" (Vref bp)
+        \prepost{(qb:Qp) (bv:N)} bp |-> primR "int" qb bv
+        \arg{gp} "gcd_result" (Vref gp)
+        \pre{garbage1:N} gp |-> primR "int" 1 garbage1
+        \arg{lp} "lcm_result" (Vref lp)
+        \pre{garbage2:N} lp |-> primR "int" 1 garbage2
+        \post emp
+      ).
+
+  cpp.spec "gcd(unsigned int, unsigned int)" as gcd_spec with (
+        \arg{a:Z} "a" (Vint a)
+        \arg{b:Z} "b" (Vint b)
+        \post [Vint (Z.gcd a b)] emp
+      ).
+
+  cpp.spec "gcd(const unsigned int&, const unsigned int&, unsigned int&)" as gcd2_spec with (
+        \arg{ap} "a" (Vref ap)
+        \prepost{(qa:Qp) (av:N)} ap |-> primR "int" qa av
+        \arg{bp} "b" (Vref bp)
+        \prepost{(qb:Qp) (bv:N)} bp |-> primR "int" qb bv
+        \arg{gp} "gcd_result" (Vref gp)
+        \pre{garbage1:N} gp |-> primR "int" 1 garbage1
+        \post gp |-> primR "int" 1 (Z.gcd av bv)
+      ).
+
+  Definition thread_constructor (lamStructTyName: core.name) :=
+  specify
+    {|
+      info_name :=
+        Nscoped (Ninst "Thread" [Atype (Tnamed lamStructTyName)]) (Nctor [Tref (Tconst (Tnamed lamStructTyName))]);
+      info_type :=
+        tCtor (Ninst "Thread" [Atype (Tnamed lamStructTyName)])
+          [Tref (Tconst (Tnamed lamStructTyName))]
+    |}
+    (ThreadConstructor lamStructTyName).
+
+  Lemma par: denoteModule module |-- pgl.
+  Proof using.
+    verify_spec'.
+    go.
+  Abort.
+   
+  Existing Instance UNSAFE_read_prim_cancel.
+
+  Lemma par: denoteModule module ** (thread_constructor "parallel_gcd_lcm(const unsigned int&, const unsigned int&, unsigned int&, unsigned int&)::@0") ** gcd2_spec |-- pgl.
+  Proof using.
+    verify_spec'.
+    slauto.
+    aggregateRepPieces a.
+    go.
+    
+    fold cQpc.
+    (* TODO: pick a better name *)
+    iExists (gp |-> intR 1%Qp garbage1 ** ap |-> intR (qa/3) av ** bp |-> intR (qb/3) bv).
+    iExists (gp |-> intR 1%Qp (Z.gcd av bv) ** ap |-> intR (qa/3) av ** bp |-> intR (qb/3) bv).
+    go.
+    iSplitL "".
+    { verify_spec'.
+      go.
+    }
+    iIntrosDestructs.
+    slauto.
+    const.
+    go.
+    slauto.
+    go.
+    go.
+    iModIntro.
+    fwd removeLater.
+
+
+    
+cpp.spec ((Ninst
+          (Nscoped resultn
+             (Nctor
+                [Trv_ref (Tconst (Tnamed (Nscoped (Nglobal (Nid "monad")) (Nid "Receipt"))));
+                 Tnamed (Nscoped resultn (Nid "value_converting_constructor_tag"))]))
+          [Atype (Tconst (Tnamed (Nscoped (Nglobal (Nid "monad")) (Nid "Receipt")))); Atype "void"]))
+  as result_val_constr with (fun this:ptr =>
+                               \arg{recp} ("recp"%pstring) (Vref recp)
+                               \prepost{r} recp |-> ReceiptR r
+                               \arg{vtag} ("vtag"%pstring) (Vptr vtag)
+                               \post this |-> ResultSuccessR ReceiptR r).
+  
 End with_Sigma.
+(*
+- pretty printing of goal: ltac.
+- hide cQp?
+- docker image
+-  rename all Vref to Vptr?
+ *)
