monadproofs/proofs/demomisc.v
@@ -1,0 +1,74 @@
+Require Import bedrock.auto.cpp.proof.
+Require Import bedrock.auto.cpp.tactics4.
+Section with_Sigma.
+  Context `{Sigma:cpp_logic} {CU: genv}.
+
+Lemma primR_anyR_ex: ∀  (t : type) (q : cQp.t),
+    Exists v,  primR t q v ⊢ anyR t q.
+Proof using.
+  intros.
+  go.
+Qed.
+
+Lemma uncurry_post_wand (P:mpred) (Qs Q: ptr -> mpred):
+  (P -* Forall x, (Qs x-* Q x))
+    |-- (Forall x, ((P ** Qs x)-* Q x)).
+Proof. Admitted.
+
+Lemma wpl f ρ module
+  s Qs Q:
+  (Forall v, Qs v -* Q v) **  (wp f ρ s (Kreturn (λ v : ptr, Qs v))) |--
+    (wp f ρ s (Kcleanup module [] (Kreturn (λ v : ptr, |> Q v)))).
+Proof using. Admitted.
+
+End with_Sigma.
+
+Ltac clearPost :=
+  repeat match goal with
+    | H: mpred |- _ => try clear H
+    | H : ptr-> mpred |- _ => try clear H
+    end.
+
+
+Ltac verify_spec2 :=
+  work; (* NOT go as that puts Seq into the continuation as Kseq, making the next rewrite fail *)
+  try rewrite uncurry_post_wand; (* TODO: make it work only the hyp of the form -* POST v *)
+  rewrite <- wpl;
+  eagerUnifyU; (* this does not suffice: see split_spec proof. need to do evar tricks to infer Qs *)
+  work;
+  name_locals;
+  cpp.hints.type.has_type_prop_prep;
+  try clearPost.
+
+Ltac verify_spec1 :=
+  IPM.perm_left ltac:(fun L n =>
+                        match L with 
+                        denoteModule ?module  =>
+                          iApply (verify_spec_new false false false module with ""%string);
+                            [vm_compute; reflexivity|]
+
+                        end
+                     ).
+
+Ltac verify_spec :=
+  iIntrosDestructs;
+  verify_spec1;
+  verify_spec2.
+
+Ltac runUntilPost :=
+  match goal with
+    |- context[Kreturn ?post] => hideFromWork post
+  end;
+  go;
+  unhideAllFromWork;
+  repeat rewrite <- primR_tptsto_fuzzyR.
+
+Ltac hideLoc l :=
+  IPM.perm_left ltac:(fun t n=>
+                        match t with
+                        | l |-> ?r => hideFromWork r
+                        end
+
+                     ).
+
+
